test-suite/SPropTests.v
@@ -1,0 +1,26 @@
+Require Import PeanoNat.
+
+Require Import Template.Ast.
+Require Import Template.Template.
+Require Import Template.Checker.
+Require Import String.
+
+Inductive sle (n : nat) : nat -> SProp :=
+  sle_n : sle n n
+| sle_S : forall m : nat, sle n m -> sle n (S m).
+
+Quote Recursively Definition q_sle := (sle 0 0).
+
+Example relevance_irrel : relevance_of_type (fst q_sle) nil (snd q_sle) = RelOk Irrelevant.
+Proof. reflexivity. Qed.
+
+Quote Recursively Definition q_arrow := (nat -> nat).
+
+Example relevance_rel: relevance_of_type (fst q_arrow) nil (snd q_arrow) = RelOk Relevant.
+Proof. reflexivity. Qed.
+
+Quote Recursively Definition q_id := (fun (x : nat) => x).
+
+Example relevance_not_sort :
+  exists a, relevance_of_type (fst q_id) nil (snd q_id) = RelNotSort a.
+Proof. eexists. reflexivity. Qed.
